Hashmap/DHashMap/AdditionalOperations.lean
@@ -1,0 +1,27 @@
+/-
+Copyright (c) 2024 Lean FRO, LLC. All rights reserved.
+Released under Apache 2.0 license as described in the file LICENSE.
+Authors: Markus Himmel
+-/
+import Hashmap.DHashMap.WF
+
+/-!
+This file defines operations on `DHashMap` which cannot be defined in `Basic.lean` due to universe issues.
+This file will have more imports than `Basic.lean` once everything is properly untangled.
+-/
+
+set_option autoImplicit false
+
+universe u v w
+
+variable {α : Type u} {β : α → Type v} {γ : Type w} {δ : α → Type w}
+
+namespace MyLean.DHashMap
+
+def filterMap [BEq α] [Hashable α] (f : (a : α) → β a → Option (δ a)) (m : DHashMap α β) : DHashMap α δ :=
+  ⟨Raw₀.filterMap f ⟨m.1, m.2.size_buckets_pos⟩, .wf (Raw₀.filterMap f ⟨m.1, m.2.size_buckets_pos⟩).2 m.2.out.filterMap⟩
+
+def map [BEq α] [Hashable α] (f : (a : α) → β a → δ a) (m : DHashMap α β) : DHashMap α δ :=
+  ⟨Raw₀.map f ⟨m.1, m.2.size_buckets_pos⟩, .wf (Raw₀.map f ⟨m.1, m.2.size_buckets_pos⟩).2 m.2.out.map⟩
+
+end MyLean.DHashMap
